nasty unsatisfaction

examples/data_structures/graph/Seq.Complements.fst
@@ -7,13 +7,13 @@ let ( @^ ) (s:seq 'a) (i:_in s) : 'a = index s i
 let snoc (s:seq 'a) (x:'a) = s `append` (create 1 x)
 
 let rec index_of_aux (#a:eqtype) (e:a) (s : seq a) (i : _in s)
- : Pure (option (_in s)) 
-  (requires (count e (slice s 0 i) == 0)) 
+ : Pure (option (_in s))
+  (requires (count e (slice s 0 i) == 0))
   (ensures fun i' -> match i' with | None -> count e s == 0 | Some i0 -> s @^ i0 == e)
   (decreases (length s - i))
 = if s @^ i = e
   then Some i
-  else begin 
+  else begin
     lemma_eq_elim (slice s 0 (i + 1)) (append (slice s 0 i) (slice s i (i + 1)));
     lemma_append_count_aux e (slice s 0 i) (slice s i (i + 1));
     assert(count e (slice s 0 (i+1)) == 0);
@@ -27,7 +27,47 @@ let rec index_of_aux (#a:eqtype) (e:a) (s : seq a) (i : _in s)
   end
 
 let index_of(#a:eqtype) (e:a) (s : seq a)
- : Pure (option (_in s)) 
+ : Pure (option (_in s))
   (requires (True))
   (ensures fun i' -> match i' with | None -> count e s == 0 | Some i0 -> s @^ i0 == e)
   = if length s = 0 then None else index_of_aux e s 0
+
+let rec index_of_l_aux (#a:Type) (f:a -> bool) (s:seq a) (i:_in s)
+  : Tot (option (_in s)) (decreases (length s - i))
+= if f (s @^ i) then Some i else if i = length s - 1 then None else index_of_l_aux #a f s (i+1)
+
+let index_of_l (#a:Type) (f:a -> bool) (s:seq a) : option (_in s) =
+  if length s = 0 then None else index_of_l_aux #a f s (0 <: _in s)
+
+let rec index_of_l_aux_spec (#a:Type) (f:a -> bool) (s:seq a) (i:_in s) :
+  Lemma (requires (forall (j:_in s{j < i}). not (f (s @^ j))))
+    (ensures (let r = index_of_l_aux f s i in
+    (forall (i:_in s). (~(Some? r) \/ i < Some?.v r) ==>  not (f (s @^ i))) /\
+      (Some? r ==> f (s @^ Some?.v r))))
+    (decreases (length s - i))
+= if f (s @^ i) then () else if i = length s - 1 then () else index_of_l_aux_spec #a f s (i+1)
+
+let rec index_of_l_spec (#a:Type) (f:a -> bool) (s:seq a) :
+    Lemma (let r = index_of_l f s in
+    (forall (i:_in s). (~(Some? r) \/ i < Some?.v r) ==> not (f (s @^ i))) /\
+      (Some? r ==> f (s @^ Some?.v r)))
+= if length s = 0 then ()
+  else index_of_l_aux_spec f s 0
+
+
+let rec none_count_zero (#a:eqtype) (e:a) (s:seq a)
+  : Lemma (requires (forall (i:_in s). not (e = s @^ i))) (ensures (count e s == 0)) (decreases (length s))
+= if length s = 0 then ()
+  else
+    let s' = tail s in
+    assert (not (e = s @^ 0)) ;
+    assert (forall (i:_in s'). not (e = s @^ (i+1))) ;
+    none_count_zero #a e s'
+
+let index_of_l_count (#a:eqtype) (e:a) (s:seq a)
+  : Lemma (match index_of_l (fun x -> x = e) s with | None -> count e s == 0 | Some i0 -> s @^ i0 = e)
+= let f x = x = e in
+  index_of_l_spec f s ;
+  match index_of_l f s with
+  | None -> none_count_zero e s
+  | Some i0 -> ()
